src/Smp.v
@@ -1,0 +1,37 @@
+From stdpp Require Import base.
+
+Class Smp P Q := { smp_smp : P ↔ Q  }.
+Class SmpHyp P Q := { smp_hyp : P → Q }.
+Class SmpHypKeep P Q := { smp_hyp_keep : P → Q }.
+Class SmpGoal P Q := { smp_goal : Q → P }.
+
+Global Hint Mode Smp + - : typeclass_instances.
+Global Hint Mode SmpHyp + - : typeclass_instances.
+
+Global Instance smp_hyp_default {P Q} `{Smp P Q} : SmpHyp P Q | 100 :=
+  {| smp_hyp := proj1 smp_smp |}.
+
+Global Instance smp_goal_default {P Q} `{Smp P Q} : SmpGoal P Q | 100 :=
+  {| smp_goal := proj2 smp_smp |}.
+
+Definition smp_rw1 `{Smp P Q} : P → Q := proj1 smp_smp.
+Definition smp_rw2 `{Smp P Q} : Q → P := proj2 smp_smp.
+
+Tactic Notation "smp" :=
+  let rec rw_hyps :=
+    try match goal with
+    | H : ?P |- _ =>
+       lazymatch type of P with
+       | Prop =>
+          let temp := fresh "temp" in
+          tryif (assert (temp:=smp_hyp_keep H)) then
+            revert temp; revert H;
+            first [rw_hyps; intros H; let H' := fresh H in intros H' | fail]
+          else
+            (try first [apply smp_hyp in H | apply smp_rw1 in H]);
+            revert H;
+            first [rw_hyps; intros H | intros H; fail 1]
+       | _ => fail
+       end
+    end in
+  try first [apply smp_goal | apply smp_rw2]; rw_hyps; simpl in *.
